\question foo
\begin{parts}
    \part bar
    \begin{solution}
        Dado $X = \{ x_1,x_2, x_3, \dots, x_n\}$

        Temos ainda que $\overline{x} = \frac{\sum{x_i}}{n}$, logo:
        \begin{equation*}
            \begin{split}
                \sum_{n}^{i = 1}{(x_i - \overline{x})^2} = \sum_{n}^{i = 1}{[x_i^2 - 2\overline{x}\sum^{n}_{i=1}{x_i} + n\overline{x}^2]} = \sum^{n}_{i=1}{x^2_i - 2n\overline{x}^2 + n\overline{x}^2} = \sum^{n}_{i=1}{x^2_i - n\overline{x}^2}
            \end{split}
        \end{equation*}
    \end{solution}

    \part bar2
    \begin{solution}
        
    \end{solution}

    \part bar3
    \begin{solution}
        A variância será calculada como:
        \begin{equation*}
            \begin{split}
                s^2 &= \frac{1}{n-1} \times \sum^{n}_{i=1}{(x_i - \overline{x}) 2} \\
                s^2 &= \frac{1}{16} \times [56.8 - 17(3.34)^2] \approx 0.502 \therefore s = \sqrt{0.502} \approx 0.71
            \end{split}
        \end{equation*}
    \end{solution}
\end{parts}